examples/low-level/ulib/FStar.StackHeap2.fst
@@ -16,8 +16,10 @@ let rec suffix_of l0 l1 =
   if List.Tot.length l0 >= List.Tot.length l1 then false
   else Cons.tl l1 = l0 || suffix_of l0 (Cons.tl l1) 
 
-let t = (id:list rid{suffix_of [root] id} & //the stack contains at least 2 elements; is that intentional?
-	 m:Map.t rid heap{forall i. List.Tot.contains i id ==> Map.contains m i})
+let is_valid_stack s = suffix_of [root] s
+
+let t = (frame_ids:list rid{is_valid_stack frame_ids} & //the stack contains at least 2 elements; is that intentional?
+	 m:Map.t rid heap{forall i. List.Tot.contains i frame_ids ==> Map.contains m i})
 
 let mem = t
 
@@ -29,6 +31,9 @@ type stacked (a:Type) =
 type rref (i:rid) (a:Type) = s:stacked a{s.id = i}
 
 let frameOf #a (s:stacked a) = s.id
+
+abstract val as_rref : #a:Type -> s:stacked a -> Tot (rref s.id a)
+let as_rref #a s = s
 
 abstract val as_ref : #a:Type -> s:stacked a -> GTot (ref a)
 let as_ref #a s = s.r
@@ -43,8 +48,8 @@ val lemma_as_ref_inj: #a:Type -> #i:rid -> r:rref i a
 let lemma_as_ref_inj #a #i r = ()
 
 (* Returns the stack of region ids *)
-val stack: t -> Tot (list rid)
-let stack s = dfst s
+val frame_ids: t -> Tot (list rid)
+let frame_ids s = dfst s
 
 (* Returns the map of heaps corresponding to the region ids *)
 val heaps: t -> Tot (Map.t rid heap)
@@ -52,29 +57,27 @@ let heaps s = dsnd s
 
 (* s0 is a suffix of of s1, hence s0's references are readable and writable from s1 *)
 abstract val is_parent: t -> t -> Tot bool
-let is_parent s0 s1 = suffix_of (stack s0) (stack s1) 
+let is_parent s0 s1 = suffix_of (frame_ids s0) (frame_ids s1) 
 
 (* Current frame id *)
 val top_frame_id: s:t -> Tot rid
-let top_frame_id s = Cons.hd (stack s)
+let top_frame_id s = Cons.hd (frame_ids s)
 
 (* Current allocatable heap *)
-val top_frame: s:t{stack s <> []} -> Tot heap
+val top_frame: s:t{frame_ids s <> []} -> Tot heap
 let top_frame s = Map.sel (heaps s) (top_frame_id s)
 
 (* Valid heap (the root frame is an ancestor *)
-(* THIS LOOKS DODGY: 
-     1. given the type of t, this should always be true
-     2. if you do pop something under this condition, you may no longer have a t
+(* CHANGED THIS:
+     Basically, it's poppable if it's valid after popping
 *)     
-//let valid (s:t) = includes [root] (stack s) \/ stack s = [root]
-let poppable (s:t) = suffix_of [root] (stack s)
+//let valid (s:t) = includes [root] (frame_ids s) \/ frame_ids s = [root]
+let poppable (s:t) = is_valid_stack (Cons.tl (dfst s))
 
 (* s1 has a new frame on top of s0. JK: Because of maps monotonicity I believe it 
    guaranties the unicity of the new frame id, needs to be checked *)
 let fresh_frame (s0:t) (s1:t) = 
-  suffix_of [root] (stack s1) /\        //this clause seems trivial from the type of t 
-  Cons.tl (stack s1) = stack s0 /\      //the new stack extends the old one by just one frame
+  Cons.tl (frame_ids s1) = frame_ids s0 /\      //the new stack extends the old one by just one frame
   not (Map.contains (heaps s0) (top_frame_id s1)) /\ //this new frame is not anywhere in the old stack
   (heaps s1 = Map.upd (heaps s0) (top_frame_id s1) emp) //and the new frame's heap is empty
 
@@ -82,17 +85,17 @@ let fresh_frame (s0:t) (s1:t) =
 let modifies (s:Set.set rid) (m0:t) (m1:t) =
   Map.equal (heaps m1) (Map.concat (heaps m1) (Map.restrict (Set.complement s) (heaps m0)))
 
-let modifies_top (m0:t) (m1:t) = stack m0 = stack m1 /\ modifies (Set.singleton (top_frame_id m1)) m0 m1
+let modifies_top (m0:t) (m1:t) = frame_ids m0 = frame_ids m1 /\ modifies (Set.singleton (top_frame_id m1)) m0 m1
 
 (* s01 is popped into s1 *)
 let popped_stack (s0:t) (s1:t) =
-  suffix_of [root] (stack s0) /\  //again, seems vacuous
-  Cons.tl (stack s0) = stack s1 /\ 
+  suffix_of [root] (frame_ids s0) /\  //again, seems vacuous
+  Cons.tl (frame_ids s0) = frame_ids s1 /\ 
   modifies Set.empty s1 s0
 
 let sel_rref (#a:Type) (#i:rid) (m:t) (r:rref i a) : a = Heap.sel (Map.sel (heaps m) i) (as_ref r)
 let upd_rref (#a:Type) (#i:rid) (m:t) (r:rref i a) (v:a) : t = 
-  (|stack m,  Map.upd (heaps m) i (Heap.upd (Map.sel (heaps m) i) (as_ref r) v)|)
+  (|frame_ids m,  Map.upd (heaps m) i (Heap.upd (Map.sel (heaps m) i) (as_ref r) v)|)
 
 let sel (#a:Type) (m:t) (r:stacked a) : a = sel_rref #a #r.id m r 
 let upd (#a:Type) (m:t) (r:stacked a) (v:a) : t = upd_rref #a #r.id m r v
@@ -111,7 +114,7 @@ val lemma_modifies_trans: m1:t -> m2:t -> m3:t
 let lemma_modifies_trans m1 m2 m3 s1 s2 = ()
 
 let contains_rref (#a:Type) (#i:rid) (r:rref i a) (m:t) =
-    List.Tot.contains i (stack m) && Heap.contains (Map.sel (heaps m) i) (as_ref r)
+    List.Tot.contains i (frame_ids m) && Heap.contains (Map.sel (heaps m) i) (as_ref r)
 
 let contains (#a:Type) (m:t) (r:stacked a) =
   contains_rref #a #r.id r m
@@ -124,7 +127,7 @@ val upd_lemma: #a:Type -> s0:t -> s1:t -> x:stacked (FStar.Seq.seq a) -> j:nat -
 	(ensures (j < Seq.length (sel s0 x) /\ sel s1 x = Seq.upd (sel s0 x) j tmpi))
 let upd_lemma #a s0 s1 x j tmpi = ()	
   
-let contains_frame (m:t) (id:rid) = List.Tot.contains id (stack m)
+let contains_frame (m:t) (id:rid) = List.Tot.contains id (frame_ids m)
 
 let fresh_rref (#a:Type) (#i:rid) (r:rref i a) (m0:t) (m1:t) =
   not (contains_rref r m0) /\ contains_rref r m1
